# F04: Propositional Logic: Boolean Algebra


* [Skill Description](#skill-description)
* [Sample Problems](#Sample-Problems)
* [Skill Tutorial](#Tutorial)
* [Answers to Sample Problems](#Answers)
* [Further Reading](#Reading)

---

# Skill Description

The ability to apply the rules of boolean algebra to transform propositional formulas into equivalent formulas. In particular, to be able to 
* convert a formula to Conjunctive Normal Form or Disjunctive Normal Form
* move all negations down to the propositional symbols
* convert a formula so it only uses and, or, and not.

---

# Sample Problems

## Problem 1

Simplify $(A\rightarrow B) \rightarrow \neg (B \rightarrow A)$ by transforming it to a formula containing only the and, or, and not operators.


## Problem 2

Simplify $\neg (P \rightarrow (Q \rightarrow P))$  by transforming it to a formula containing only the and, or, and not operators.


---

# Tutorial

Any formula in propositional logic can be reduced to one containing only the $\vee$ and $\wedge$ operators
and propositional symbols $P,Q,...$ and their negations $\neg P, \neg Q, \ldots$.
r

## Precedence and Associativity
Propositional Formulas are easier to read if they are not fully parenthesized. Just as with the PEMDAS rules for
arithmetic (parentheses, exponents, multiplication, division, addition, subtraction), we have precedence rules
for propositional formulas with the following order
* parentheses override all precedence $P \wedge (Q \vee R)$
* negation binds tightest $\neg P$
* conjunction is next $P \wedge Q$
* disjunction and xor are next $P \vee Q$ and $P \oplus Q$
* implication is next $P \rightarrow Q$
* iff is the weakest $P \leftrightarrow Q$


Also, if there are multiple operators of the same precedence in a row then they associate to the left except for $\rightarrow$ and $\leftrightarrow$ which associate to the right, e.g.
* $P \vee Q \oplus R \vee S$ is interpreted as $((P \vee Q) \oplus R) \vee S$
* $P \rightarrow Q \rightarrow R\rightarrow S$ is interpreted as $P \rightarrow (Q \rightarrow (R\rightarrow S))$

So $P \wedge Q \vee R \wedge S \leftrightarrow T \leftrightarrow \neg R \wedge V$ would be fully parenthesized as
$$((P \wedge Q) \vee (R \wedge S)) \leftrightarrow (T \leftrightarrow ((\neg R) \wedge V))$$


## Simplification rules
To do this, we use the DeMorgan rules to push negation down to the propositionial symbols,
but first we use the following substitution rules which preserve logical equivalence to remove all operators
except disjunction and conjunction:

$E \rightarrow F \equiv (\neg E \vee F)$

$E \oplus F \equiv E\wedge \neg F \vee \neg E\wedge F$

$E \leftrightarrow F \equiv E\wedge F \vee (\neg E)\wedge (\neg F)$

## Example
Lets show how to simplify $P \rightarrow (Q \rightarrow  R\oplus P)$

This example doesn't require any use of the DeMorgan rules.

First we remove the implications and the exclusive or using the simplication rules

$P \rightarrow (Q \rightarrow  R\oplus P) \equiv$

$P \rightarrow (Q \rightarrow  R\wedge \neg P \vee \neg R\wedge P) \equiv$

$P \rightarrow (\neg Q \vee  R\wedge \neg P \vee \neg R\wedge P) \equiv$

$\neg P \vee (\neg Q \vee  R\wedge \neg P \vee \neg R\wedge P) \equiv$

$(\neg P )\vee (\neg Q) \vee  (R\wedge \neg P) \vee (\neg R\wedge P)$ .... parentheses added for clarity...

and this is a disjunction of conjuctions of propositional symbols or their negations,
i.e. it is in Disjunctive Normal Form (DNF).

So this is true in four cases:
1. P is False
2. Q is false
3. R is true and P is false
4. R is false and P is true

and we could easily use this to write out the Truth Table of the formula.




## Simplifying Negations of formulas
In this section, we give some examples of simiplifying the negation of a formula
by using using the DeMorgan rules to move the negation symbols all the way in to the formula
so the only negations are those on primitive propositional symbols.

Being able to accurately perform these simplifications is important in proving properties of logical formulas!

## Example
Let's simplify $\neg(P\wedge Q \rightarrow R)$
The first step is to replace the implication $A\rightarrow B$ with an equivalent disjunction $\neg A \vee B$, so

$\neg(P\wedge Q \rightarrow R) \equiv \neg(\neg(P\wedge Q) \vee R)$

then we apply DeMorgan to either the outer disjunction or the inner conjuction. Let simpify the inner negation first:

$\neg(\neg(P\wedge Q) \vee R) \equiv \neg ( \neg P \vee \neg Q \vee R)$

Now we can simplify the outer negation:

$\neg ( \neg P \vee \neg Q \vee R) \equiv P \wedge Q \wedge \neg R$

Notice were using a slight generalization of the DeMorgan Law wich states that the negation of a disjunction 
is the conjunction of negations of its elements. We have shown than

$\neg(P\wedge Q \rightarrow R) \equiv  P \wedge Q \wedge \neg R$

You can test the equivalence of these with Truth Tables if you want.



## Generalized DeMorgan's Law
There is a useful generalization of DeMorgan's Law that works for any formula containing only $\vee$, $\wedge$, $\neg$ and propositional symbols.

Let $F$ be any such formula and let $\overline{F}$ be the fully parenthesized formula obtained by replacing all $\vee$ with $\wedge$ and $\wedge$ with $\vee$ and replacing each propositional symbol $P$ with its negation $\neg P$, and replacing $true$ with $false$ and vice versa. Then

$\neg F = \overline{F}$

For example, if 

$F = P \vee \neg (Q \wedge \neg R) \vee (\neg P \wedge Q)$, then

$\neg F = \neg P \wedge (Q \wedge \neg R) \vee (\neg P \wedge Q)$

$\neg F = \neg P \wedge \neg (\neg Q \vee  R) \wedge  ( P \vee \neg Q)))$

and you can verify for yourself using DeMorgan that $\neg F = \overline{F}$

## Theorem proving by simplifying negation
One approach to proving that a boolean formula $F$ is valid, i.e. is a tautology, is to show that the
negation of the formula $\neg F$ simplifies to False; or equivalently, using the booolean algebra rules
to show that $F$ is equivalent to True, that is, 

$\neg F \equiv {\rm false}$   -->  $F \equiv {\rm true}$

In many cases this is much faster than using the Truth Table method to show $F$ is true for all interpretation, but there is no known "fast" algorithm to prove a formula is a tautology.


---

# Answers

## Problem 1

Simplify $(A\rightarrow B) \rightarrow \neg (B \rightarrow A)$

**Answer:**
First we replace the implications with disjunctions:

$(A\rightarrow B) \rightarrow \neg (B \rightarrow A) \equiv$

$(\neg A\vee B) \rightarrow \neg (\neg B \vee A) \equiv$

$\neg (\neg A\vee B) \vee \neg (\neg B \vee A) \equiv$

Then we apply the DeMorgan rules:

$(\neg\neg A\wedge \neg B) \vee (\neg\neg B \wedge \neg A) \equiv$

and we remove the double negations as $\neg\neg A \equiv A$

$(A\wedge \neg B) \vee (B \wedge \neg A)$

and this says that exactly one of A and B is True, so this expressions is equivalent to $A\oplus B$

## Problem 2

Simplify $\neg (P \rightarrow (Q \rightarrow P))$

**Answer:**
First we replace the implications $A\rightarrow B$ with disjunctions $\neg A \vee B$:

$\neg (P \rightarrow (Q \rightarrow P)) \equiv \neg (P \rightarrow (\neg Q \vee P)) \equiv \neg (\neg P \vee (\neg Q \vee P))$

Using DeMorgan we get

$\neg (\neg P \vee (\neg Q \vee P)) \equiv \neg\neg P \wedge \neg(\neg Q \vee P)$

Next we apply DeMorgan again to get 

$\neg\neg P \wedge \neg(\neg Q \vee P) \equiv \neg\neg P \wedge \neg\neg Q \wedge \neg P$

Since double negation is the identity, $\neg\neg P\equiv P$, we get 

$\neg\neg P \wedge \neg\neg Q \wedge \neg P \equiv P \wedge Q \wedge \neg P$

but $P \wedge \neg P \equiv False$ and $False \wedge Q \equiv False$, so the entire formula
simplifes to False, and we have shown that

$\neg (P \rightarrow (Q \rightarrow P)) \equiv False$

In other words $\neg (P \rightarrow (Q \rightarrow P))$ is unsatisfiable, 
and by negating both sides we see also that

$P \rightarrow (Q \rightarrow P) \equiv True$

So $P\rightarrow (Q \rightarrow P)$ is a valid formula, i.e. a taugology.

---

# Reading
