# G05: Generating Functions


* [Skill Description](#skill-description)
* [Sample Problems](#Sample-Problems)
* [Skill Tutorial](#Tutorial)
* [Answers to Sample Problems](#Answers)
* [Further Reading](#Reading)

---


# Skill Definition
The ability to use Generating Functions to find closed form solutions to recurrence equations.



---

# Sample-Problems

## Problem 1
Use the Generating Function method to find the closed form for the recurrence defined by

$s_0=2$, $s_1=1$ and

$s_n = s_{n-1} + 6 s_{n-2}$ for all $n\ge 2$



## Problem 2
Use the Generating Function method to find the closed form for the recurrence defined by

$s_0=1$ $s_1=6$

$s_n = 6 s_{n-1} - 9s_{n-2}$ for all $n\ge 2$


---

# Tutorial

One of the most powerful techniques for finding a closed form for the elements of a recursively defined sequences
it to use the sequence $s$ to create a function $f_s(x)$ and to show how the recursion equation on $s$ translates
into properties of the function $f_s(x)$. We can the use those properties to find a closed form for the coefficients
of the function, which give a formula for the original sequence!

## Definition of the Generating Function for a Sequence
Let $s = (s_0,s_1,\ldots)$ be an infinite sequence of numbers,
then we can associated to $s$ a powerseries $f_s$ (i.e. an infinite degree polynomial)  defined by

$$f_s(x) = \sum_{i=0}^\infty s_i x^i = s_0 + s_1x + s_2x^2 + s_3x^3 + s_4x^4 + \ldots$$

## constant sequence
if $s=(1,1,1,\ldots)$ then 

$$f_s(x) = 1 + x + x^2 + x^3 + \ldots = \sum_\limits{n=0}^\infty x^n$$

and 

$f_s(x) = 1/(1-x)$.

To see this we can show that $1 = (1-x) f_s(x) = f_s(x) - x*f_s(x)$

$$f_s(x) = 1 + x + x^2 + x^3 + \ldots$$

$$xf_s(x) = x + x^2 + x^3 + x^4 + \ldots$$

$$f_s(x) - xf_s(x) =1 + x + x^2 + x^3 + \ldots -  (x + x^2 + x^3 + x^4 + \ldots) = 1$$


## geometric sequence
if $s = (1,t,t^2,t^3,\ldots, t^k,\ldots)$ then  

$$f_s(x) = 1 + tx + t^2x^2 + t^3x^3 + \ldots = \sum_\limits{n=0}^\infty t^nx^n$$

and 

$f_s(x) = 1/(1-tx)$

and we can see this by substituting $tx$ for $x$ in the formula for the constant sequence...

## Generalized Binomial Theorem
If $s_k = \binom{r}{k}$ then 

$$f_s(x) = \sum_\limits{k=0}^\infty \binom{r}{k} x^k = (1+x)^r$$

where $\binom{r}{k} = \frac{r * (r-1) * \ldots * (r-k+1)}{k!}$ holds for all real values of $r$ including negative and positive real numbers, not just positive integers!

We won't prove this here... the simplest proof requires knowing about Taylor series and differentiation which isn't a prereq for this course (but is very cool stuff!)

### Example of using the Generalized Binomial Theorem
e.g.
* with $r=-2$
  * $\binom{-2}{0}= 1$
  * $\binom{-2}{1}= -2/1$
  * $\binom{-2}{2}= \frac{-2 * -3}{1 * 2} = 3$
  * $\binom{-2}{3}= \frac{-2 * -3 * -4}{ 1 * 2 * 3} = -4$
  * $\ldots$
  * $\binom{-2}{k}= (k+1) * (-1)^k$
  * So

$$(1+x)^{-2} = 1 - 2x +3x^2 -4x^3 + \ldots + (k+1) * (-1)^kx^k + \ldots = \sum_{k=0}^\infty (k+1)(-1)^kx^k$$

and so

$$(1-tx)^{-2} = 1 +2tx +3t^2x^2 +4t^3x^3 + \ldots + (k+1) * t^kx^k + \ldots = \sum_{k=0}^\infty (k+1)t^kx^k$$
  

## Polynomial Sequence
If $s_k=p(k)$ for some polynomial k of degree d, then

$f_s = q(x)/(1-x)^d$ where q is a polynomial of degree less than $d$

So the generating function for a polynomial sequence is always of the form $q(x)/(1-x)^d$ for some polynomial $q$

## Exponential Sequences from a recurrence relation
If $f_s$ is a powerseries in $x$, and $a$ is a number, then $g = ax f_s$ is also a powerseries and

$$
ax f_s(x) = ax\sum_{i=0}^\infty s_i x^i = as_0x + as_1x^2 + as_2x^3 + as_3x^4 + as_4x^5 + \ldots
 = \sum_{i=1}^\infty as_{i-1}x^i
$$

Likewise, 

$$
bx^2 f_s(x)  = bx^2\sum_{i=0}^\infty s_i x^i = bs_0x^2 + bs_1x^3 + bs_2x^4 + bs_3x^5 + bs_4x^6 + \ldots
 = \sum_{i=2}^\infty bs_{i-2}x^i
$$

So

$$ (1 -ax -bx^2) f_s(x) = \sum_{i=0}^\infty s_{i}x^i - \sum_{i=1}^\infty as_{i-i}x^i - \sum_{i=2}^\infty bs_{i-2}x^i
= s_0 + as_1x + \sum_{i=2}^\infty (s_i - as_{i-1}- bs_{i-2})x^i
$$

So if $s$ satisfies the recursive equation

$s_0 = u$ $s_1 = v$ and $s_i = a s_{i-1} + b s_{i-2}$ for all $i\ge 2$

Then we see that

$$(1 -ax -bx^2) f_s(x) = s_0 + as_1 x $$

and $s_0 = u$ and $as_1 = av$ and

$$f_s(x) = \frac {u + avx}{1 - ax - bx^2}$$

So if we can find a closed form for the coefficients of this, then we'll have a closed form for the sequence!

Our first step is to factor $(1-ax-bx^2) = (1-\alpha_1 x) (1 - \alpha_2 x)$
and if $\alpha_1\ne\alpha_2$ we can use polynomial interpolation to find numbers $r$ and $s$ such that

$$f_s(x) = \frac {u + avx}{1 - ax - bx^2} = \frac r {1-\alpha_1 x} + \frac s {1-\alpha_2 x}$$

but if $\alpha_1 = \alpha_2 = \alpha$ then

$$f_s(x) = \frac {u + a v x} {(1-\alpha x)^2}$$

and both of these forms have nice closed form solutions as we have seen above!

A similar argument works for linear recurrences with 3 or more terms...

## More general recurrence equations.

We'll look at more general, non-homogeneous, equations later and show how they can be solved using the Generating Function method.

---

# Answers

## Problem 1
Use the Generating Function method to find the closed form for the recurrence defined by

$s_0=2$, $s_1=1$ and

$s_n = s_{n-1} + 6 s_{n-2}$ for all $n\ge 2$

**Answer:**
We start off with $f_s$ being the generating function for the sequence $s$:

$$f_s(x) = \sum_{i=0}^\infty s_i x^i = s_0 + s_1x + s_2x^2 + s_3x^3 + s_4x^4 + \ldots $$

so

$$f_s(x) = \sum_{i=0}^\infty s_i x^i = 2 + x + s_2x^2 + s_3x^3 + s_4x^4 + \ldots = 2 + x + \sum_{i=2}^\infty s_i x^i$$


$$xf_s(x) = \sum_{i=1}^\infty s_{i-1} x^i = 0 + 2x + s_1x^2 + s_2x^3 + s_3x^4 + s_4x^5 + \ldots = 0 + 2x + + \sum_{i=2}^\infty s_{i-1} x^i$$

$$x^2f_s(x) = \sum_{i=2}^\infty s_{i-2} x^i = 0 + 0x + s_0x^2 + s_1x^3 + s_2x^4 + s_3x^5 + s_4x^6 + \ldots = 0 + 0x + \sum_{i=2}^\infty s_{i-2} x^i$$

$$(1 - x - 6x^2)f_s(x) = \sum_{i=2}^\infty s_{i-2} x^i = (2 + x) + -2x + 
\sum_{i=2}^\infty (s_i - s_{i-1} - 6 s_{i-2}) x^i  = 2-x$$

So we can express $f_s(x)$ as a quotient of polynomials and use the partial fractions approach to express it in terms of exponential series we already know:

$$ f_s(x) = \frac{2-x}{1-x-6x^2} = \frac a {1-3x} + \frac b {1+2x} = \frac {a + 2ax + b - 3bx}{(1-3x)(1+2x)}$$

So we must solve $a+b + (2a-3b)x = 2 - x$  that is $a+b=2$ and $2a-3b = -1$.

Adding 3 times the first equation to the second we get $5a = 5$ so $a=1$ and $b=1$ and

$$ f_x(x) = \frac 1 {1-3x} + \frac 1 {1 - (-2)x} = \sum_{n=0}^\infty (3^n + (-2)^n) x^n$$

which implies that $s_n = 3^n + (-2)^n$ and we have used the Generating Functions method to find a closed form
for the sequence given its linear recurrence equation.

---

## Problem 2
Use the Generating Function method to find the closed form for the recurrence defined by

$s_0=1$ $s_1=6$

$s_n = 6 s_{n-1} - 9s_{n-2}$ for all $n\ge 2$

**Answer:**
We start off with $f_s$ being the generating function for the sequence $s$:

$$f_s(x) = \sum_{i=0}^\infty s_i x^i = s_0 + s_1x + s_2x^2 + s_3x^3 + s_4x^4 + \ldots $$

so

$$f_s(x) = \sum_{i=0}^\infty s_i x^i = 1 + 6x + s_2x^2 + s_3x^3 + s_4x^4 + \ldots = 2 + x + \sum_{i=2}^\infty s_i x^i$$


$$xf_s(x) = \sum_{i=1}^\infty s_{i-1} x^i = 0 + 6x + s_1x^2 + s_2x^3 + s_3x^4 + s_4x^5 + \ldots = 0 + 2x + + \sum_{i=2}^\infty s_{i-1} x^i$$

$$x^2f_s(x) = \sum_{i=2}^\infty s_{i-2} x^i = 0 + 0x + s_0x^2 + s_1x^3 + s_2x^4 + s_3x^5 + s_4x^6 + \ldots = 0 + 0x + \sum_{i=2}^\infty s_{i-2} x^i$$

$$(1 - 6x +9x^2)f_s(x) = \sum_{i=2}^\infty s_{i-2} x^i = (1 + 6x) + -6x + 
\sum_{i=2}^\infty (s_i - 6s_{i-1} +9 s_{i-2}) x^i  = 1$$

So we can express $f_s(x)$ as a quotient of polynomials and use the partial fractions approach to express it in terms of exponential series we already know:

$$ f_s(x) = \frac{1}{1-6x+9x^2} = \frac 1 {(1-3x)^2}  = \sum_{n=0}^\infty (n+1) 3^n x^n$$

So $s_n = (n+1) 3^n$ and we have used the Generating Function Method to find a closed form for the nth element of this sequence defined by a linear recursion.





